Reorganize

FloatModel/Model/Format/Basic.lean
@@ -9,7 +9,7 @@ module
 -- need to rely on.
 @[expose] public section
 
-namespace FloatModel
+namespace Float.Model
 
 def totalExponent (mantissa : Nat) (exponent : Int) :=
   mantissa.log2 + 1 + exponent
@@ -19,7 +19,7 @@ A floating point format is specified by two pieces of information: the number
 of bits in the mantissa, and the range of the exponent, which is represented by
 the exponent that denotes infinity.
 -/
-structure FloatSpec where
+structure Format where
   /-- The number of bits in the mantissa, *excluding the implicit bit*. -/
   mantissaBitsWithoutImplicit : Nat
   hm : 0 < mantissaBitsWithoutImplicit := by decide
@@ -27,42 +27,42 @@ structure FloatSpec where
   exponentBits : Nat
   he : 0 < exponentBits := by decide
 
-namespace FloatSpec
+namespace Format
 
 /-- Specification corresponding to the IEEE `binary32` format. -/
-abbrev binary32 : FloatSpec where
+abbrev binary32 : Format where
   mantissaBitsWithoutImplicit := 23
   exponentBits := 8
 
 /-- Specification corresponding to the IEEE `binary64` format. -/
-abbrev binary64 : FloatSpec where
+abbrev binary64 : Format where
   mantissaBitsWithoutImplicit := 52
   exponentBits := 11
 
 /-- The total number of bits in the packed representation. -/
-abbrev numBits (spec : FloatSpec) : Nat :=
+abbrev numBits (spec : Format) : Nat :=
   1 + spec.exponentBits + spec.mantissaBitsWithoutImplicit
 
 /-- The number of bits in the mantisse, *including the implicit bit*. -/
-def mantissaBits (spec : FloatSpec) : Nat :=
+def mantissaBits (spec : Format) : Nat :=
   1 + spec.mantissaBitsWithoutImplicit
 
 /-- The exponent that represents the infinities. -/
-def infinityExponent (spec : FloatSpec) : Nat :=
+def infinityExponent (spec : Format) : Nat :=
   2 ^ (spec.exponentBits - 1)
 
 /--
 The exponent bias. In packed formats, we store the sum of the true exponent and
 the bias.
 -/
-def exponentBias (spec : FloatSpec) : Nat :=
+def exponentBias (spec : Format) : Nat :=
   2 ^ (spec.exponentBits - 1) - 1
 
 /--
 The smallest exponent possible for a number using the given specification,
 including subnormals.
 -/
-def minExponent (spec : FloatSpec) : Int :=
+def minExponent (spec : Format) : Int :=
   3 - spec.infinityExponent - spec.mantissaBits
 
 /--
@@ -70,16 +70,16 @@ Suppose we have written a number where `totalExponent` is the position of the
 most significant digit with the unit digit corresponds to `1`. So, for example,
 `1.0b` has total exponent `1`, `0.1b` has total exponent `0`, `0.01b` has total
 exponent `-1`, and so on. This function computes which exponent that number
-should have according to the given `FloatSpec`. So, for example, for the number
+should have according to the given `Format`. So, for example, for the number
 `0.1b` in `binary64` format, it wants us to use the exponent `-53`, corresponding
 to the representation `2^52 * 2^(-53)`, which has a 53-bit mantissa. If the total
 exponent gets quite small, then the result exponent eventually gets capped at
 `spec.minExponent`, which first forces the result to be a subnormal number and
 then, if the total exponent is even smaller, to be zero.
 -/
-def targetExponent (spec : FloatSpec) (totalExponent : Int) : Int :=
+def targetExponent (spec : Format) (totalExponent : Int) : Int :=
   max (totalExponent - spec.mantissaBits) spec.minExponent
 
-end FloatSpec
+end Format
 
-end FloatModel
+end Float.Model
