FloatModel/Contrib/Misc.lean
@@ -1,0 +1,49 @@
+/-
+Copyright (c) 2026 Lean FRO, LLC. All rights reserved.
+Released under Apache 2.0 license as described in the file LICENSE.
+Authors: Julia M. Himmel
+-/
+module
+
+/-!
+Miscellaneous lemmas about `Nat`, `BitVec`, etc. that are used throughout the model but
+are not specific to floating-point numbers.
+-/
+
+@[expose] public section
+
+namespace Float.Model
+
+@[simp]
+theorem BitVec.toNat_pos {n : Nat} (b : BitVec n) : 0 < b.toNat ↔ 0#_ < b := by
+  simp [BitVec.lt_def]
+
+theorem BitVec.pos_iff_ne_zero {n : Nat} (b : BitVec n) : 0#_ < b ↔ b ≠ 0#_ := by
+  rw [BitVec.lt_def, Ne, ← BitVec.toNat_inj, BitVec.toNat_zero, Nat.pos_iff_ne_zero]
+
+theorem Nat.eq_iff_testBit_eq {n m : Nat} : n = m ↔ ∀ i, Nat.testBit n i = Nat.testBit m i := by
+  refine ⟨?_, Nat.eq_of_testBit_eq⟩
+  rintro rfl
+  simp
+
+@[simp]
+theorem Nat.or_pos {n m : Nat} : 0 < n ||| m ↔ 0 < n ∨ 0 < m := by
+  simp [Nat.pos_iff_ne_zero]
+  simp [Nat.eq_iff_testBit_eq]
+  simp [Decidable.imp_iff_or_not, exists_or, or_comm]
+
+@[simp]
+theorem Nat.shiftLeft_pos {n m : Nat} : 0 < n <<< m ↔ 0 < n := by
+  simp [Nat.pos_iff_ne_zero]
+
+@[simp]
+theorem BitVec.zero_eq_neg_one_iff {w : Nat} : 0#w = (-1#w) ↔ w = 0 := by
+  simp [← BitVec.toNat_inj]
+  match w with
+  | 0 => simp
+  | w + 1 =>
+    suffices 0 ≠ 2 ^ (w + 1) - 1 by simpa
+    have : 2 ≤ 2 ^ (w + 1) := Nat.le_pow (by simp)
+    omega
+
+end Float.Model
