FloatModel/Model/Float.lean
@@ -1,0 +1,51 @@
+/-
+Copyright (c) 2026 Lean FRO, LLC. All rights reserved.
+Released under Apache 2.0 license as described in the file LICENSE.
+Authors: Julia M. Himmel
+-/
+module
+
+public import FloatModel.Model.Format.Valid
+public import FloatModel.Model.Unpacked.Pack.Lemmas
+public import FloatModel.Model.Unpacked.Operations
+
+-- This file is part of the logical model for floats which authors of float libraries
+-- need to rely on.
+@[expose] public section
+
+/-- The logical model for the `Float` type. -/
+structure Float.Model where
+  /-- The underlying bit pattern of the `Float`. -/
+  toBits : UInt64
+  /-- The underlying bit pattern is valid according to the format. -/
+  valid : Float.Model.Format.binary64.Valid toBits.toBitVec
+
+namespace Float.Model
+
+/-- Unpack a `Float.Model` into the corresponding `UnpackedFloat`. -/
+def unpack (f : Float.Model) : UnpackedFloat :=
+  UnpackedFloat.unpack Format.binary64 f.toBits.toBitVec
+
+/--
+Pack an `UnpackedFloat` into the corresponding `Float.Model`.
+This operation only gives a meaningful result if the float is
+already correctly rounded for the `Format.binary64` format.
+-/
+def pack (f : UnpackedFloat) : Float.Model where
+  toBits := UInt64.ofBitVec (UnpackedFloat.pack Format.binary64 f)
+  valid := by simp
+
+/--
+Compute the sum of two `Float.Model`.
+-/
+def add (a b : Float.Model) : Float.Model :=
+  pack (UnpackedFloat.add Format.binary64 a.unpack b.unpack)
+
+/--
+Construct a `Float.Model` from its bit representation. This operation canonicalizes
+all `NaN` inputs into the canonical `NaN`.
+-/
+def ofBits (a : UInt64) : Float.Model :=
+  pack (UnpackedFloat.unpack Format.binary64 a.toBitVec)
+
+end Float.Model
