FloatModel/Model/Float32.lean
@@ -1,0 +1,19 @@
+/-
+Copyright (c) 2026 Lean FRO, LLC. All rights reserved.
+Released under Apache 2.0 license as described in the file LICENSE.
+Authors: Julia M. Himmel
+-/
+module
+
+public import FloatModel.Model.Format.Valid
+
+-- This file is part of the logical model for floats which authors of float libraries
+-- need to rely on.
+@[expose] public section
+
+/-- The logical model for the `Float32` type. -/
+structure Float32.Model where
+  /-- The underlying bit pattern of the `Float32`. -/
+  toBits : UInt32
+  /-- The underlying bit pattern is valid according to the format. -/
+  valid : Float.Model.Format.binary32.Valid toBits.toBitVec
