FloatModel/Model/Unpacked/Operations.lean
@@ -1,0 +1,15 @@
+/-
+Copyright (c) 2026 Lean FRO, LLC. All rights reserved.
+Released under Apache 2.0 license as described in the file LICENSE.
+Authors: Julia M. Himmel
+-/
+module
+
+public import FloatModel.Model.Unpacked.Operations.Add
+public import FloatModel.Model.Unpacked.Operations.Mul
+public import FloatModel.Model.Unpacked.Operations.Sub
+public import FloatModel.Model.Unpacked.Operations.Div
+public import FloatModel.Model.Unpacked.Operations.Sqrt
+public import FloatModel.Model.Unpacked.Operations.Compare
+public import FloatModel.Model.Unpacked.Operations.Sign
+public import FloatModel.Model.Unpacked.Operations.Status
